floyd/forward.v
@@ -1486,29 +1486,75 @@ tac_if (ptr_compare e) ltac:forward_ptr_cmp ltac:forward_setx.
 
 (* BEGIN new semax_load and semax_store tactics *************************)
 
-Ltac new_instantiate P Q R Rnow Delta e ids tts sh ids0 v n N H:=
- match Rnow with
+Ltac try_instantiate_load P Q R0 Delta e ids tts sh ids0 v n N H SH IDS V:=
+      assert (PROPx P (LOCALx (tc_environ Delta :: Q) (SEPx (R0 :: nil))) 
+         |-- (`(field_at sh (typeof e) ids0 v) (eval_lvalue e))) as H;
+      [unfold sh, ids0, v;
+       instantiate (2 := IDS);
+       assert (IDS = skipn (length ids - length IDS) ids) as _ by reflexivity;
+       simpl skipn; subst e ids tts;
+       instantiate (2 := SH);
+       instantiate (1 := V);
+       try unfold field_at_;
+       generalize V;
+       intro;
+       solve [(entailer!; cancel)]
+      | pose N as n ].
+
+Ltac new_instantiate_load P Q R Rnow Delta e ids tts sh ids0 v n N H:=
+  match Rnow with
   | ?R0 :: ?Rnow' => 
     match R0 with
     | `(field_at ?SH _ ?IDS ?V _) =>
-      assert (PROPx P (LOCALx (tc_environ Delta :: Q) (SEPx (R0 :: nil))) 
-         |-- (`(field_at sh (typeof e) ids0 v) (eval_lvalue e))) as H;
-      [unfold sh, ids0, v; subst e ids tts; 
-       instantiate (2 := IDS);
-       instantiate (2 := SH);
-       instantiate (1 := V);
-       solve [(entailer!; cancel)]
-      | pose N as n ]
+      try_instantiate_load P Q R0 Delta e ids tts sh ids0 v n N H SH IDS V
     | `(field_at ?SH _ ?IDS ?V) _ => 
+      try_instantiate_load P Q R0 Delta e ids tts sh ids0 v n N H SH IDS V
+    | `(field_at_ ?SH ?TY ?IDS _) =>
+      try_instantiate_load P Q R0 Delta e ids tts sh ids0 v n N H SH IDS 
+      (default_val (nested_field_type2 TY IDS))
+    | `(field_at_ ?SH ?TY ?IDS) _ => 
+      try_instantiate_load P Q R0 Delta e ids tts sh ids0 v n N H SH IDS 
+      (default_val (nested_field_type2 TY IDS))
+    | _ => new_instantiate_load P Q R Rnow' Delta e ids tts sh ids0 v n (S N) H
+    end
+  end.
+
+Ltac try_instantiate_store P Q R0 Delta e ids tts sh ids0 v n N H SH TY IDS V:=
       assert (PROPx P (LOCALx (tc_environ Delta :: Q) (SEPx (R0 :: nil))) 
-         |-- (`(field_at sh (typeof e) ids0 v) (eval_lvalue e))) as H;
-      [unfold sh, ids0, v; subst e ids tts; 
+         |-- (`(field_at sh (typeof e) ids0) v (eval_lvalue e))) as H;
+      [unfold sh, ids0, v;
        instantiate (2 := IDS);
+       assert (IDS = skipn (length ids - length IDS) ids) as _ by reflexivity;
+       simpl skipn; subst e ids tts;
        instantiate (2 := SH);
        instantiate (1 := V);
+       try unfold field_at_;
+       try rewrite <- (@liftx1_liftx0 val mpred);
+       try rewrite <- (@liftx2_liftx1 (reptype (nested_field_type2 TY IDS)) val mpred);
+       simpl typeof;
+       simpl reptype;
+       generalize V;
+       intro;
        solve [(entailer!; cancel)]
-      | pose N as n ]
-    | _ => new_instantiate P Q R Rnow' Delta e ids tts sh ids0 v n (S N) H
+      | pose N as n ].
+
+Ltac new_instantiate_store P Q R Rnow Delta e ids tts sh ids0 v n N H:=
+  match Rnow with
+  | ?R0 :: ?Rnow' => 
+    match R0 with
+    | `(field_at ?SH ?TY ?IDS ?V _) =>
+      try_instantiate_store P Q R0 Delta e ids tts sh ids0 v n N H SH TY IDS (` V)
+    | `(field_at ?SH ?TY ?IDS ?V) _ => 
+      try_instantiate_store P Q R0 Delta e ids tts sh ids0 v n N H SH TY IDS (` V)
+    | `(field_at ?SH ?TY ?IDS) ?V _ => 
+      try_instantiate_store P Q R0 Delta e ids tts sh ids0 v n N H SH TY IDS V
+    | `(field_at_ ?SH ?TY ?IDS _) =>
+      try_instantiate_store P Q R0 Delta e ids tts sh ids0 v n N H SH TY IDS 
+      (`(default_val (nested_field_type2 TY IDS)))
+    | `(field_at_ ?SH ?TY ?IDS) _ => 
+      try_instantiate_store P Q R0 Delta e ids tts sh ids0 v n N H SH TY IDS 
+      (`(default_val (nested_field_type2 TY IDS)))
+    | _ => new_instantiate_store P Q R Rnow' Delta e ids tts sh ids0 v n (S N) H
     end
   end.
 
@@ -1523,7 +1569,6 @@ Proof.
  normalize.
 Qed.
 Definition force_eq ( x y: val) := force_ptr x = force_ptr y.
-
 
 Lemma force_force_eq:
   forall v, force_ptr (force_ptr v) = force_ptr v.
@@ -1568,6 +1613,7 @@ Ltac new_load_tac :=   (* matches:  semax _ _ (Sset _ (Efield _ _ _)) _  *)
      pose (Struct env := @abbreviate _ empty_ti)
  end; 
  match goal with   
+(*
  | Struct_env := @abbreviate type_id_env _ 
    |- semax ?Delta _ (Sset _ (Efield ?e _ _)) _ =>
  match e with
@@ -1602,7 +1648,49 @@ Ltac new_load_tac :=   (* matches:  semax _ _ (Sset _ (Efield _ _ _)) _  *)
    | try apply I; try assumption; reflexivity
    ]
  end
-| SE := @abbreviate type_id_env.type_id_env _ 
+*)
+| SE := @abbreviate type_id_env _ 
+    |- semax ?Delta (|> (PROPx ?P (LOCALx ?Q (SEPx ?R)))) (Sset _ (Ecast ?e _)) _ =>
+    let pp := fresh "pp" in
+    let e1 := fresh "e" in
+    let ids := fresh "ids" in
+    let tts := fresh "tts" in
+              pose (compute_nested_efield e) as pp;
+              simpl in pp;
+              pose (fst (fst pp)) as e1;
+              pose (snd (fst pp)) as ids;
+              pose (snd pp) as tts;
+              simpl in e1, ids, tts;
+              change e with (nested_efield e1 ids tts);
+              clear pp;
+    let sh := fresh "sh" in evar (sh: share);
+    let ids0 := fresh "ids" in evar (ids0: list ident);
+    let v := fresh "v" in evar (v: reptype (nested_field_type2 (typeof e1) ids0));
+    let n := fresh "n" in
+    let H := fresh "H" in
+   
+    new_instantiate_load P Q R R Delta e1 ids tts sh ids0 v n (0%nat) H;
+    let ids1 := fresh "ids" in
+    let tts0 := fresh "tts" in
+    let tts1 := fresh "tts" in
+    pose (firstn (length ids - length ids0) ids) as ids1;
+    pose (skipn (length ids - length ids0) tts) as tts0;
+    pose (firstn (length ids - length ids0) tts) as tts1;
+    simpl in ids1, tts0, tts1;
+    change ids with (ids1 ++ ids0);
+    change tts with (tts1 ++ tts0);
+    subst ids tts;
+    let Heq := fresh "H" in
+    match type of H with
+    | (PROPx _ (LOCALx _ (SEPx (?R0 :: nil))) 
+           |-- _) => assert (nth_error R n = Some R0) as Heq by reflexivity
+    end;
+    eapply (semax_nested_efield_field_cast_load_37' Delta sh SE);
+      [reflexivity | reflexivity | solve [(simpl; auto)] | reflexivity 
+      | reflexivity | reflexivity | reflexivity
+      | apply andp_right; [|apply (nth_error_SEP_sepcon_TT _ _ _ _ _ _ H Heq)]];
+    unfold e1, ids0, ids1, tts0, tts1; solve [entailer!]
+| SE := @abbreviate type_id_env _ 
     |- semax ?Delta (|> (PROPx ?P (LOCALx ?Q (SEPx ?R)))) (Sset _ ?e) _ =>
     let pp := fresh "pp" in
     let e1 := fresh "e" in
@@ -1622,7 +1710,7 @@ Ltac new_load_tac :=   (* matches:  semax _ _ (Sset _ (Efield _ _ _)) _  *)
     let n := fresh "n" in
     let H := fresh "H" in
    
-    new_instantiate P Q R R Delta e1 ids tts sh ids0 v n (0%nat) H;
+    new_instantiate_load P Q R R Delta e1 ids tts sh ids0 v n (0%nat) H;
     let ids1 := fresh "ids" in
     let tts0 := fresh "tts" in
     let tts1 := fresh "tts" in
@@ -1632,7 +1720,7 @@ Ltac new_load_tac :=   (* matches:  semax _ _ (Sset _ (Efield _ _ _)) _  *)
     simpl in ids1, tts0, tts1;
     change ids with (ids1 ++ ids0);
     change tts with (tts1 ++ tts0);
-    clear ids tts;
+    subst ids tts;
     let Heq := fresh "H" in
     match type of H with
     | (PROPx _ (LOCALx _ (SEPx (?R0 :: nil))) 
@@ -1643,6 +1731,7 @@ Ltac new_load_tac :=   (* matches:  semax _ _ (Sset _ (Efield _ _ _)) _  *)
       | reflexivity | reflexivity | reflexivity
       | apply andp_right; [|apply (nth_error_SEP_sepcon_TT _ _ _ _ _ _ H Heq)]];
     unfold e1, ids0, ids1, tts0, tts1; solve [entailer!]
+(*
  | SE := @abbreviate type_id_env _ 
     |- semax ?Delta _ (Sset _ (Efield _ _ _)) _ =>
   eapply (semax_load_field'') with (e := SE);
@@ -1658,12 +1747,14 @@ Ltac new_load_tac :=   (* matches:  semax _ _ (Sset _ (Efield _ _ _)) _  *)
    | solve [entailer; simpl_data_at; unfold at_offset; simpl; cancel]
    | try apply I; try assumption; reflexivity
    ]
+*)
  | |- semax _ _ (Sset _ (Ederef (Ebinop Oadd ?e1 ?e2 _) _)) _ =>
     eapply semax_load_array with (lo:=0)(v1:=eval_expr e1)(v2:=eval_expr e2);
       [ reflexivity | reflexivity | entailer ]
  | |- semax _ _ (Sset _ (Ecast (Ederef (Ebinop Oadd ?e1 ?e2 _) _) _)) _ =>
     eapply semax_cast_load_array with (lo:=0)(v1:=eval_expr e1)(v2:=eval_expr e2);
       [ reflexivity | simpl; auto | entailer ]
+(*
  | SE := @abbreviate type_id_env _ |- semax _ _ (Sset _ ?e) _ =>
    let pp := fresh "pp" in
    match e with
@@ -1680,6 +1771,7 @@ Ltac new_load_tac :=   (* matches:  semax _ _ (Sset _ (Efield _ _ _)) _  *)
              | reflexivity | reflexivity | reflexivity | reflexivity 
              | reflexivity | solve [(entailer!; simpl; auto)]]
    end
+*)
  | |- _ => eapply semax_cast_load_37';
    [reflexivity 
    |entailer;
@@ -1808,6 +1900,48 @@ match goal with
   clear n sh contents lo hi ;
   [reflexivity | solve [auto] | reflexivity | auto | reflexivity |
    solve [(entailer!; try apply I; try tauto; reflexivity)]| entailer]
+| SE := @abbreviate type_id_env.type_id_env _ 
+    |- semax ?Delta (|> (PROPx ?P (LOCALx ?Q (SEPx ?R)))) (Sassign ?e _) _ =>
+    let pp := fresh "pp" in
+    let e1 := fresh "e" in
+    let ids := fresh "ids" in
+    let tts := fresh "tts" in
+              pose (compute_nested_efield e) as pp;
+              simpl in pp;
+              pose (fst (fst pp)) as e1;
+              pose (snd (fst pp)) as ids;
+              pose (snd pp) as tts;
+              simpl in e1, ids, tts;
+              change e with (nested_efield e1 ids tts);
+              clear pp;
+    let sh := fresh "sh" in evar (sh: share);
+    let ids0 := fresh "ids" in evar (ids0: list ident);
+    let v := fresh "v" in evar (v: environ -> reptype (nested_field_type2 (typeof e1) ids0));
+    let n := fresh "n" in
+    let H := fresh "H" in
+   
+    new_instantiate_store P Q R R Delta e1 ids tts sh ids0 v n (0%nat) H;
+    let ids1 := fresh "ids" in
+    let tts0 := fresh "tts" in
+    let tts1 := fresh "tts" in
+    pose (firstn (length ids - length ids0) ids) as ids1;
+    pose (skipn (length ids - length ids0) tts) as tts0;
+    pose (firstn (length ids - length ids0) tts) as tts1;
+    simpl in ids1, tts0, tts1;
+    change ids with (ids1 ++ ids0);
+    change tts with (tts1 ++ tts0);
+    subst ids tts;
+    let Heq := fresh "H" in
+    match type of H with
+    | (PROPx _ (LOCALx _ (SEPx (?R0 :: nil))) 
+           |-- _) => assert (nth_error R n = Some R0) as Heq by reflexivity
+    end;
+    eapply (semax_nested_efield_field_store_nth Delta sh SE n);
+    [reflexivity | reflexivity | simpl; auto | reflexivity
+    | reflexivity | reflexivity | exact Heq | exact H | auto | solve[entailer!] ]
+(*
+
+
 | SE := @abbreviate type_id_env _ 
     |- semax ?Delta (|> (PROPx ?P (LOCALx ?Q (SEPx ?R)))) (Sassign ?e _) _ =>
        let pp := fresh "pp" in
@@ -1850,6 +1984,8 @@ match goal with
    [reflexivity | simpl; auto | reflexivity | reflexivity | reflexivity
    | solve [entailer!] | auto | try solve [entailer!]];
   unfold n,sh; clear n sh (**** 21.1 seconds to here *****)
+*)
+
   | |- @semax ?Espec ?Delta (|> PROPx ?P (LOCALx ?Q (SEPx ?R))) 
                      (Sassign ?e ?e2) _ =>
 
