progs/verif_nest2.v
@@ -34,9 +34,11 @@ Lemma body_get:  semax_body Vprog Gprog f_get get_spec.
 Proof.
 start_function.
 name i _i.
+rewrite data_at_field_at.
 forward.
 simpl proj_reptype.
 forward.
+rewrite data_at_field_at.
 apply derives_refl.
 Qed.
 
@@ -44,7 +46,9 @@ Lemma body_set:  semax_body Vprog Gprog f_set set_spec.
 Proof.
  start_function.
 name i_ _i.
+rewrite data_at_field_at.
 forward.
 forward.
+rewrite data_at_field_at.
 entailer!.
 Qed.
